Unify different maps into a common Valuation Record.

CrIdentifiers.v
@@ -1,4 +1,5 @@
 Require Import Strings.String.
+From MyProject Require Export Map.
 
 (* Define the different types of identifiers in the Caracara DSL *)
 Inductive ParserState : Type := ParserStateCtr (name : string).
@@ -7,8 +8,27 @@ Inductive StateVar : Type := StateVarCtr (name : string).
 Inductive ModuleName : Type := ModuleNameCtr (name : string).
 Inductive FunctionName : Type := FunctionNameCtr (name : string).
 Inductive ConnectionName : Type := ConnectionNameCtr (name : string).
-Inductive VariableName : Type := VariableNameCtr (name : string).
 Inductive CtrlPlaneConfigName : Type := CtrlPlaneConfigNameCtr (name : string).
+
+(* Current values for each of these identifiers as a map *)
+Definition HeaderMap := fmap Header nat.
+Definition StateVarMap := fmap StateVar nat.
+Definition CtrlPlaneConfigNameMap := fmap CtrlPlaneConfigName nat.
+
+(* The valuation is a record containing three maps:,
+   one each for mapping headers/statevars/ctrlplaneconfigs to their current values *)
+Record Valuation := {
+  ctrl_plane_map : CtrlPlaneConfigNameMap;
+  header_map : HeaderMap;
+  state_var_map : StateVarMap
+}.
+
+(* Empty valuation *)
+Example empty_valuation : Valuation := {|
+  ctrl_plane_map := empty CtrlPlaneConfigName nat;
+  header_map := empty Header nat;
+  state_var_map := empty StateVar nat
+|}.
 
 (* example of parser state *)
 Definition example_parser_state := ParserStateCtr "example_parser_state".
