CrSemantics.v
@@ -6,23 +6,10 @@ Require Import Strings.String.
 From MyProject Require Export CrIdentifiers.
 From MyProject Require Export Map.
 
-(* Headers and states (or rather their valuations) are both represented
-   as maps from names of headers and state variables to their values expressed as integers *)
-Definition HeaderMap := fmap Header nat.
-Definition StateMap := fmap StateVar nat.
-
-(* InputType is the input to the transformer, which is a pair of previous header and previous state *)
-(* OutputType is the output of the transformer, which is a pair of new header and new state *)
-Definition HeaderStatePair := (HeaderMap * StateMap)%type.
-
-(* Empty header state pair *)
-Example header_state_pair_example : HeaderStatePair := (empty Header nat, empty StateVar nat).
-
 (* TODO: fill out eval_transformer body at the end,
    right now, we are just specifying it as a function that
-   goes from previous value of header+state
-   to new value of header+state *)
-Parameter eval_transformer : Transformer -> HeaderStatePair -> HeaderStatePair.
+   goes from previous valuation to new one *)
+Parameter eval_transformer : Transformer -> Valuation -> Valuation.
 
 (* A Transformer is a list of match-action rules,
    where each rule is either sequential or parallel,
@@ -31,22 +18,34 @@ Parameter eval_transformer : Transformer -> HeaderStatePair -> HeaderStatePair.
 (* Function to evaluate a match-action rule,
    meaning header ops within an action are evaluated
    according to the type of the rule (sequential or parallel) *)
-Parameter eval_match_action_rule : MatchActionRule -> HeaderStatePair -> HeaderStatePair.
+Parameter eval_match_action_rule : MatchActionRule -> Valuation -> Valuation.
 
 (* Function to evaluate a sequential match-action rule,
    meaning header ops within an action are evaluated sequentially *)
-Parameter eval_seq_rule : MatchActionRule -> HeaderStatePair -> HeaderStatePair.
+Parameter eval_seq_rule : MatchActionRule -> Valuation -> Valuation.
 
 (* Function to evaluate a parallel match-action rule,
    meaning header ops within an action are evaluated in parallel *)
-Parameter eval_par_rule : MatchActionRule -> HeaderStatePair -> HeaderStatePair.
+Parameter eval_par_rule : MatchActionRule -> Valuation -> Valuation.
 
 (* Function to evaluate a header operation,
-   meaning we apply the operation to the header and state *)
-Definition eval_hdr_op (op : HdrOp) (input : HeaderStatePair) : HeaderStatePair :=
+   meaning we apply the operation to a previous valuation to get a new one *)
+Definition eval_hdr_op (op : HdrOp) (input_valuation : Valuation) : Valuation :=
     match op with
-    | StatefulOp f arg1 arg2 target => header_state_pair_example (* Placeholder for actual evaluation logic *)
-    | StatelessOp f arg1 arg2 target => header_state_pair_example (* Placeholder for actual evaluation logic *)
+    | StatefulOp f arg1 arg2 target =>
+        let new_state :=
+           let op_output := f (function_argument_to_nat arg1 input_valuation) (function_argument_to_nat arg2 input_valuation) in
+            add (state_var_map input_valuation) target op_output in
+            {| ctrl_plane_map := ctrl_plane_map input_valuation;   (* Leave this unchanged *)
+               header_map := header_map input_valuation; (* Leave this unchanged *)
+               state_var_map := new_state |}           (* Modify this *)
+    | StatelessOp f arg1 arg2 target =>
+        let new_hdr :=
+           let op_output := f (function_argument_to_nat arg1 input_valuation) (function_argument_to_nat arg2 input_valuation) in
+            add (header_map input_valuation) target op_output in
+            {| ctrl_plane_map := ctrl_plane_map input_valuation;   (* Leave this unchanged *)
+               header_map := new_hdr; (* Modify this *)
+               state_var_map := state_var_map input_valuation |}  (* Leave this unchanged *)
     end.
 
 (*TODO: Maybe figure out a way to unify parsing and header manipulation into seq and par transformers respectively. *)
